src/cardinality/sc_amo.lean
@@ -1,5 +1,5 @@
 /-
-The Sinz at-most-one encoding.
+The sequential counter at-most-one encoding.
 
 Authors: Cayden Codel, Jeremy Avigad, Marijn Heule
 Carnegie Mellon University
@@ -20,7 +20,7 @@ import data.nat.basic
 
 variables {V : Type*} [inhabited V] [decidable_eq V]
 
-namespace sinz_amo
+namespace sc_amo
 
 open nat
 open list
@@ -47,7 +47,7 @@ variables {l : list (literal V)} {g : gensym V}
   if (0 < i) then [[Neg (g.nth (i - 1)), lit.flip]] else []
 
 -- TODO: no need to case on length 0 and 1, because the length checks handle things?
-def sinz_amo : enc_fn V
+def sc_amo : enc_fn V
 | []     g := ⟨[], g⟩
 | [lit₁] g := ⟨[], g⟩
 | l      g :=
@@ -76,12 +76,12 @@ begin
       exact ih (le_of_lt_succ (lt_of_le_of_ne Hi hn)) } }
 end
 
-theorem xi_to_si_mem_sinz_amo (g : gensym V) {i : nat} (Hi : i < length l - 1) (Hi' : i < length l) :
-  [(l.nth_le i Hi').flip, Pos (g.nth i)] ∈ (sinz_amo l g).1 :=
+theorem xi_to_si_mem_sc_amo (g : gensym V) {i : nat} (Hi : i < length l - 1) (Hi' : i < length l) :
+  [(l.nth_le i Hi').flip, Pos (g.nth i)] ∈ (sc_amo l g).1 :=
 begin
   cases l with lit₁ ls, { simp at Hi, contradiction },
   cases ls with lit₂ ls, { simp at Hi, contradiction },
-  rw sinz_amo,
+  rw sc_amo,
   simp at Hi Hi',
   simp [-map_with_index_cons],
   use [((xi_to_si g (ls.length + 2) i ((lit₁ :: lit₂ :: ls).nth_le i Hi')) ++ 
@@ -94,11 +94,11 @@ begin
 end
 
 theorem si_to_next_si_mem (g : gensym V) {i : nat} (Hi : i < length l - 2) :
-  [Neg (g.nth i), Pos (g.nth (i + 1))] ∈ (sinz_amo l g).1 :=
+  [Neg (g.nth i), Pos (g.nth (i + 1))] ∈ (sc_amo l g).1 :=
 begin
   cases l with lit₁ ls, { simp at Hi, contradiction },
   cases ls with lit₂ ls, { simp at Hi, contradiction },
-  rw sinz_amo,
+  rw sc_amo,
   simp at Hi,
   have Hi' : i < length (lit₁ :: lit₂ :: ls),
   { simp, exact lt_succ_of_lt (lt_succ_of_lt Hi) },
@@ -112,11 +112,11 @@ begin
 end
 
 theorem si_to_next_xi_mem (g : gensym V) {i : nat} (Hi : i + 1 < length l) :
-  [Neg (g.nth i), (l.nth_le (i + 1) Hi).flip] ∈ (sinz_amo l g).1 :=
+  [Neg (g.nth i), (l.nth_le (i + 1) Hi).flip] ∈ (sc_amo l g).1 :=
 begin
   cases l with lit₁ ls, { simp at Hi, contradiction },
   cases ls with lit₂ ls, { simp at Hi, contradiction },
-  rw sinz_amo,
+  rw sc_amo,
   have Hi' : i < length (lit₁ :: lit₂ :: ls),
   { simp at Hi, simp only [length], exact lt_succ_of_lt Hi },
   simp [-map_with_index_cons],
@@ -130,20 +130,20 @@ end
 
 -- If the var is in l, then use τ.
 -- Otherwise, the signal variable is true if at least 1 variable before is true
-def sinz_amo_tau (l : list (literal V)) (g : gensym V) (τ : assignment V) : assignment V :=
+def sc_amo_tau (l : list (literal V)) (g : gensym V) (τ : assignment V) : assignment V :=
   aite (clause.vars l) τ (λ v, (alk 1).eval τ (l.take ((var_idx g v (length l - 1)) + 1)))
 
-theorem sinz_amo_eval_tt_under_sinz_amo_tau (hdis : disj l g) : ∀ (τ : assignment V), 
-  (amk 1).eval τ l = tt → (sinz_amo l g).1.eval (sinz_amo_tau l g τ) = tt :=
+theorem sc_amo_eval_tt_under_sc_amo_tau (hdis : disj l g) : ∀ (τ : assignment V), 
+  (amk 1).eval τ l = tt → (sc_amo l g).1.eval (sc_amo_tau l g τ) = tt :=
 begin
   intros τ heval,
   cases l with lit₁ ls,
-  { simp [sinz_amo] },
+  { simp [sc_amo] },
   cases ls with lit₂ ls,
-  { simp [sinz_amo] },
+  { simp [sc_amo] },
   { rw eval_tt_iff_forall_clause_eval_tt,
     intros c hc,
-    rw sinz_amo at hc,
+    rw sc_amo at hc,
     unfold prod.fst at hc,
     simp [-map_with_index_cons] at hc,
     rcases hc with ⟨f, ⟨lit, i, ⟨hi, rfl⟩, rfl⟩, hmemc⟩,
@@ -157,12 +157,12 @@ begin
         cases halk : (alk 1).eval τ ((lit₁ :: lit₂ :: ls).take (i + 1)),
         { use [((lit₁ :: lit₂ :: ls).nth_le i hi).flip, mem_cons_self _ _],
           simp [eval_flip],
-          rw [sinz_amo_tau, aite_pos_lit (mem_vars_of_mem (nth_le_mem (lit₁ :: lit₂ :: ls) i hi))],
+          rw [sc_amo_tau, aite_pos_lit (mem_vars_of_mem (nth_le_mem (lit₁ :: lit₂ :: ls) i hi))],
           have hamk : !((alk 1).eval τ ((lit₁ :: lit₂ :: ls).take (i + 1))) = !ff, exact congr_arg bnot halk,
           rw [← amk_eval_eq_alk_succ_eval, bool.bnot_ff, amz_eval_tt_iff_forall_eval_ff] at hamk,
           exact hamk (nth_le_mem_take_of_lt hi (lt_succ_self i)) },
         { use [Pos (g.nth i), mem_cons_of_mem _ (mem_singleton_self _)],
-          rw [literal.eval, sinz_amo_tau, aite_neg (disj_right.mp hdis (nth_mem_stock g i)), var_idx_eq_nth_of_le],
+          rw [literal.eval, sc_amo_tau, aite_neg (disj_right.mp hdis (nth_mem_stock g i)), var_idx_eq_nth_of_le],
           { exact halk },
           { simp only [length, succ_add_sub_one], exact le_of_lt_succ hi } } } },
     { unfold si_to_next_si at hc,
@@ -171,13 +171,13 @@ begin
         rw eval_tt_iff_exists_literal_eval_tt,
         cases halk : (alk 1).eval τ ((lit₁ :: lit₂ :: ls).take (i + 1)),
         { use [Neg (g.nth i), mem_cons_self _ _],
-          rw [literal.eval, sinz_amo_tau, aite_neg (disj_right.mp hdis (nth_mem_stock g i)), var_idx_eq_nth_of_le],
+          rw [literal.eval, sc_amo_tau, aite_neg (disj_right.mp hdis (nth_mem_stock g i)), var_idx_eq_nth_of_le],
           { have hamk : !((alk 1).eval τ ((lit₁ :: lit₂ :: ls).take (i + 1))) = !ff, exact congr_arg bnot halk,
             rw [← amk_eval_eq_alk_succ_eval, bool.bnot_ff] at hamk,
             rw ← amk_eval_eq_alk_succ_eval, exact hamk },
           { simp only [length, succ_add_sub_one], exact le_of_lt_succ hi } },
         { use [Pos (g.nth (i + 1)), mem_cons_of_mem _ (mem_singleton_self _)],
-          rw [literal.eval, sinz_amo_tau, aite_neg (disj_right.mp hdis (nth_mem_stock g (i + 1))), var_idx_eq_nth_of_le],
+          rw [literal.eval, sc_amo_tau, aite_neg (disj_right.mp hdis (nth_mem_stock g (i + 1))), var_idx_eq_nth_of_le],
           { rw alk.eval_tt_of_sublist_of_eval_tt (take_sublist_of_le (le_succ (i + 1)) _),
             { exact halk },
             { exact _inst_1 } },
@@ -190,13 +190,13 @@ begin
         rw eval_tt_iff_exists_literal_eval_tt,
         cases halk : (alk 1).eval τ ((lit₁ :: lit₂ :: ls).take (i + 1)),
         { use [Neg (g.nth i), mem_cons_self _ _],
-          rw [literal.eval, sinz_amo_tau],
+          rw [literal.eval, sc_amo_tau],
           rw [aite_neg (disj_right.mp hdis (nth_mem_stock g i)), var_idx_eq_nth_of_le],
           { rw bnot_eq_true_eq_eq_ff, exact halk },
           { simp only [length, succ_add_sub_one], exact le_of_lt_succ (lt_of_succ_lt hi) } },
         { use [((lit₁ :: lit₂ :: ls).nth_le i.succ hi).flip, mem_cons_of_mem _ (mem_singleton_self _)],
           simp [-nth_le, eval_flip],
-          rw [sinz_amo_tau, aite_pos_lit (mem_vars_of_mem (nth_le_mem (lit₁ :: lit₂ :: ls) _ hi))],
+          rw [sc_amo_tau, aite_pos_lit (mem_vars_of_mem (nth_le_mem (lit₁ :: lit₂ :: ls) _ hi))],
           have hi' : i.succ < (lit₁ :: lit₂ :: ls).length, exact hi,
           rw amo_eval_tt_iff_distinct_eval_ff_of_eval_tt at heval,
           rcases alo_eval_tt_iff_exists_eval_tt.mp halk with ⟨z, hmem, hevalz⟩,
@@ -205,16 +205,16 @@ begin
           exact heval this hevalz } } } }
 end
 
-theorem sinz_amo_mem_vars {l : list (literal V)} {g : gensym V} :
-  ∀ ⦃v⦄, v ∈ (sinz_amo l g).1.vars → v ∈ (clause.vars l) ∨ (v ∈ (g.nfresh (length l - 1)).1) :=
+theorem sc_amo_mem_vars {l : list (literal V)} {g : gensym V} :
+  ∀ ⦃v⦄, v ∈ (sc_amo l g).1.vars → v ∈ (clause.vars l) ∨ (v ∈ (g.nfresh (length l - 1)).1) :=
 begin
   -- redo proof with si_to_si_mem theorems?
   cases l with lit₁ ls,
-  { simp [sinz_amo] },
+  { simp [sc_amo] },
   { cases ls with lit₂ ls,
-    { simp [sinz_amo] },
+    { simp [sc_amo] },
     { intros v hv,
-      rw sinz_amo at hv,
+      rw sc_amo at hv,
       unfold prod.fst at hv,
       simp [-map_with_index_cons] at hv,
       rcases hv with ⟨F, ⟨lit, idx, ⟨hlen, rfl⟩, rfl⟩, hf⟩,
@@ -247,40 +247,40 @@ begin
           { exact or.inl (mem_vars_of_mem (mem_cons_of_mem _ (nth_le_mem _ _ _))) } } } } }
 end
 
-theorem sinz_amo_is_wb : is_wb (sinz_amo : enc_fn V) :=
+theorem sc_amo_is_wb : is_wb (sc_amo : enc_fn V) :=
 begin
   intros l g hdis,
   cases l with lit₁ ls,
-  { simp [sinz_amo] },
+  { simp [sc_amo] },
   cases ls with lit₂ ls,
-  { simp [sinz_amo] },
+  { simp [sc_amo] },
   { split,
-    { rw sinz_amo,
+    { rw sc_amo,
       intros v hv,
       simp only [prod.snd] at hv,
       exact (nfresh_stock_subset _ _) hv },
     { intros v hv,
       apply (set.mem_union _ _ _).mpr,
-      rcases sinz_amo_mem_vars hv with (hv | hv),
+      rcases sc_amo_mem_vars hv with (hv | hv),
       { exact or.inl hv },
       { exact or.inr ⟨nfresh_mem_stock hv, nth_not_mem_nfresh_stock hv⟩ } } }
 end
 
 theorem signal_eval_tt_if_xi_eval_tt {i : nat} {hi : i < length l}
   (hi' : i < length l - 1) :
-  (sinz_amo l g).1.eval τ = tt → (l.nth_le i hi).eval τ = tt → τ (g.nth i) = tt :=
+  (sc_amo l g).1.eval τ = tt → (l.nth_le i hi).eval τ = tt → τ (g.nth i) = tt :=
 begin
   cases l with lit₁ ls, { simp only [length, not_lt_zero'] at hi, contradiction },
   cases ls with lit₂ ls, { simp only [length_singleton, not_lt_zero'] at hi', contradiction },
   intros heval hlit,
   rw eval_tt_iff_forall_clause_eval_tt at heval,
-  have := heval _ (xi_to_si_mem_sinz_amo g hi' hi),
+  have := heval _ (xi_to_si_mem_sc_amo g hi' hi),
   simp [eval_tt_iff_exists_literal_eval_tt, eval_flip, literal.eval, hlit] at this,
   exact this
 end
 
 theorem signal_eval_tt_of_prev_signal_eval_tt {i : nat} (hi : i < length l - 2) :
-  (sinz_amo l g).1.eval τ = tt → 
+  (sc_amo l g).1.eval τ = tt → 
   τ (g.nth i) = tt → ∀ ⦃j : nat⦄, (j > i ∧ j < length l - 1) → τ (g.nth j) = tt :=
 begin
   cases l with lit₁ ls, { simp only [length, not_lt_zero'] at hi, contradiction },
@@ -302,7 +302,7 @@ begin
 end
 
 theorem nth_eval_ff_of_signal_eval_tt {i : nat} (hi : i < length l - 1) :
-  (sinz_amo l g).1.eval τ = tt → τ (g.nth i) = tt → 
+  (sc_amo l g).1.eval τ = tt → τ (g.nth i) = tt → 
   ∀ {j : nat} (hj : (j > i) ∧ (j < length l)), (l.nth_le j hj.2).eval τ = ff :=
 begin
   cases l with lit₁ ls, { simp only [length, not_lt_zero'] at hi, contradiction },
@@ -323,17 +323,17 @@ begin
       exact hc } }
 end
 
-theorem sinz_amo_formula_encodes : is_correct (amk 1) (sinz_amo : enc_fn V) :=
+theorem sc_amo_formula_encodes : is_correct (amk 1) (sc_amo : enc_fn V) :=
 begin
   intros l g hdis τ,
   cases l with lit₁ ls,
-  { simp [sinz_amo] },
+  { simp [sc_amo] },
   { cases ls with lit₂ ls,
-    { simp [sinz_amo], use τ },
+    { simp [sc_amo], use τ },
     { split,
       { intro hamk,
-        use [(sinz_amo_tau (lit₁ :: lit₂ :: ls) g τ), sinz_amo_eval_tt_under_sinz_amo_tau hdis τ hamk],
-        intros v hv, rw [sinz_amo_tau, aite_pos hv] },
+        use [(sc_amo_tau (lit₁ :: lit₂ :: ls) g τ), sc_amo_eval_tt_under_sc_amo_tau hdis τ hamk],
+        intros v hv, rw [sc_amo_tau, aite_pos hv] },
       { rintros ⟨σ, hs, hagree_on⟩,
         rw amo_eval_tt_iff_distinct_eval_ff_of_eval_tt,
         rintros lit₁ lit₂ ⟨i, j, hi, hj, hij, rfl, rfl⟩ hl₁,
@@ -348,7 +348,7 @@ end
 -- Alernative proof of reverse direction using the amk semantics directly
 /-
 
-theorem signal_semantics₁ : (sinz_amo l g).1.eval τ = tt → 
+theorem signal_semantics₁ : (sc_amo l g).1.eval τ = tt → 
   ∀ ⦃i : nat⦄, i < length l - 1 → τ (g.nth i) = ff → (amk 0).eval τ (l.take (i + 1)) = tt :=
 begin
   cases l with lit₁ ls, { simp },
@@ -357,7 +357,7 @@ begin
   rw eval_tt_iff_forall_clause_eval_tt at heval,
   induction i with i ih,
   { have : 0 < (lit₁ :: lit₂ :: ls).length, { simp },
-    have := heval _ (xi_to_si_mem_sinz_amo g hi this),
+    have := heval _ (xi_to_si_mem_sc_amo g hi this),
     simp [literal.eval, eval_flip, htau] at this,
     simp [this] },
   { cases htau' : τ (g.nth i),
@@ -367,7 +367,7 @@ begin
       { rw [amk.eval_take_tail_neg hlit, take],
         simp at ih hi,
         exact ih (lt_of_succ_lt hi) htau' },
-      { have := heval _ (xi_to_si_mem_sinz_amo g hi hi'),
+      { have := heval _ (xi_to_si_mem_sc_amo g hi hi'),
         rw nth_le at hlit,
         simp [literal.eval, eval_flip, htau, hlit] at this,
         contradiction } },
@@ -378,7 +378,7 @@ begin
       contradiction } }
 end
 
-theorem signal_semantics₂ : (sinz_amo l g).1.eval τ = tt →
+theorem signal_semantics₂ : (sc_amo l g).1.eval τ = tt →
   ∀ ⦃i : nat⦄, i < length l - 1 → τ (g.nth i) = tt → (amk 1).eval τ (l.take (i + 1)) = tt :=
 begin
   cases l with lit₁ ls, { simp },
@@ -432,21 +432,21 @@ end
       contradiction } }
 -/
 
-theorem sinz_amo_encodes_amo : encodes (amk 1) (sinz_amo : enc_fn V) :=
-⟨sinz_amo_formula_encodes, sinz_amo_is_wb⟩ 
+theorem sc_amo_encodes_amo : encodes (amk 1) (sc_amo : enc_fn V) :=
+⟨sc_amo_formula_encodes, sc_amo_is_wb⟩ 
 
 -- The version easier for theorem proving
-def sinz_amo_rec : enc_fn V
+def sc_amo_rec : enc_fn V
 | []                   g := ⟨[], g⟩
 | [lit₁]               g := ⟨[], g⟩
 | [lit₁, lit₂]         g := ⟨[[lit₁.flip, Pos g.fresh.1], [Neg g.fresh.1, lit₂.flip]], g.fresh.2⟩
 | (lit₁ :: lit₂ :: ls) g :=
   ⟨[[lit₁.flip, Pos g.fresh.1], [Neg g.fresh.1, Pos g.fresh.2.fresh.1], [Neg g.fresh.1, lit₂.flip]] ++ 
-   (sinz_amo_rec (lit₂ :: ls) g.fresh.2).1,
-   (sinz_amo_rec (lit₂ :: ls) g.fresh.2).2⟩
+   (sc_amo_rec (lit₂ :: ls) g.fresh.2).1,
+   (sc_amo_rec (lit₂ :: ls) g.fresh.2).2⟩
 
--- A nicer looking and more efficient presentation of the Sinz encoding
-def sinz_amo_rec' : enc_fn V
+-- A nicer looking and more efficient presentation of the sc encoding
+def sc_amo_rec' : enc_fn V
 | []                   g := ⟨[], g⟩
 | [lit₁]               g := ⟨[], g⟩
 | [lit₁, lit₂]         g := 
@@ -455,12 +455,12 @@ def sinz_amo_rec' : enc_fn V
 | (lit₁ :: lit₂ :: ls) g :=
     let ⟨y, g₁⟩ := g.fresh in
     let ⟨z, _⟩ := g₁.fresh in
-    let ⟨F_rec, g₂⟩ := sinz_amo_rec' (lit₂ :: ls) g₁ in
+    let ⟨F_rec, g₂⟩ := sc_amo_rec' (lit₂ :: ls) g₁ in
     ⟨[[lit₁.flip, Pos y], [Neg y, Pos z], [Neg y, lit₂.flip]] ++ F_rec, g₂⟩
 
--- The two definitions of the Sinz encoding are equivalent on all inputs
-theorem sinz_amo_rec_eq_sinz_amo_rec' : ∀ (l : list (literal V)) (g : gensym V),
-  sinz_amo_rec l g = sinz_amo_rec' l g :=
+-- The two definitions of the sc encoding are equivalent on all inputs
+theorem sc_amo_rec_eq_sc_amo_rec' : ∀ (l : list (literal V)) (g : gensym V),
+  sc_amo_rec l g = sc_amo_rec' l g :=
 begin
   intros l g,
   induction l with lit₁ ls ih generalizing g,
@@ -468,23 +468,23 @@ begin
   { cases ls with lit₂ ls,
     { refl },
     { cases ls with lit₃ ls,
-      { simp [sinz_amo_rec, sinz_amo_rec'], unfold fresh, refl },
-      { rw [sinz_amo_rec, sinz_amo_rec'],
-        rw [prod.ext_self g.fresh, sinz_amo_rec'._match_4,
-            prod.ext_self g.fresh.2.fresh, sinz_amo_rec'._match_3,
-            ← ih, prod.ext_self (sinz_amo_rec _ _)],
-        rw sinz_amo_rec'._match_2 } } }
+      { simp [sc_amo_rec, sc_amo_rec'], unfold fresh, refl },
+      { rw [sc_amo_rec, sc_amo_rec'],
+        rw [prod.ext_self g.fresh, sc_amo_rec'._match_4,
+            prod.ext_self g.fresh.2.fresh, sc_amo_rec'._match_3,
+            ← ih, prod.ext_self (sc_amo_rec _ _)],
+        rw sc_amo_rec'._match_2 } } }
 end
 
-theorem sinz_amo_rec_is_wb : is_wb (sinz_amo_rec : enc_fn V) :=
+theorem sc_amo_rec_is_wb : is_wb (sc_amo_rec : enc_fn V) :=
 begin
   intros l g hdis,
   induction l with lit₁ ls ih generalizing g,
-  { simp [sinz_amo_rec] },
+  { simp [sc_amo_rec] },
   { cases ls with lit₂ ls,
-    { simp [sinz_amo_rec] },
+    { simp [sc_amo_rec] },
     { cases ls with lit₃ ls,
-      { simp [sinz_amo_rec, cnf.vars, var, flip_var_eq],
+      { simp [sc_amo_rec, cnf.vars, var, flip_var_eq],
         split,
         { exact fresh_stock_subset g },
         { intros v hv,
@@ -494,7 +494,7 @@ begin
           { apply set.mem_union_left, simp only [set.mem_insert_iff, eq_self_iff_true, true_or] },
           { apply set.mem_union_right,
             exact ⟨fresh_mem_stock g, fresh_not_mem_fresh_stock g⟩ } } },
-      { rw sinz_amo_rec,
+      { rw sc_amo_rec,
         simp [cnf.vars, var, flip_var_eq],
         have ihred := ih (disj_fresh_cons hdis),
         split,
@@ -506,8 +506,8 @@ begin
           { apply set.mem_union_right, split,
             { exact fresh_fresh_mem_stock g },
             { intro hcon,
-              have : g.fresh.2.fresh.1 ∈ (sinz_amo_rec (lit₂ :: lit₃ :: ls) g.fresh.2).1.vars,
-              { cases ls with lit₄ ls; { rw sinz_amo_rec, simp [cnf.vars, var] } },
+              have : g.fresh.2.fresh.1 ∈ (sc_amo_rec (lit₂ :: lit₃ :: ls) g.fresh.2).1.vars,
+              { cases ls with lit₄ ls; { rw sc_amo_rec, simp [cnf.vars, var] } },
               rcases (set.mem_union _ _ _).mp (ihred.2 this) with (hv | hv),
               { exact (disj_left.mp (disj_of_disj_cons hdis) hv) (fresh_fresh_mem_stock g) },
               { exact hv.2 hcon } } },
@@ -526,23 +526,23 @@ begin
               exact ⟨(fresh_stock_subset g) hv.1, hv.2⟩ } } } } } }
 end
 
-theorem sinz_amo_rec_amz {l} {g} (hdis : disj l g) : (amk 0).eval τ l = tt → 
-  (sinz_amo_rec l g).1.eval (aite (clause.vars l) τ all_tt) = tt :=
+theorem sc_amo_rec_amz {l} {g} (hdis : disj l g) : (amk 0).eval τ l = tt → 
+  (sc_amo_rec l g).1.eval (aite (clause.vars l) τ all_tt) = tt :=
 begin
   induction l with lit₁ ls ih generalizing g,
-  { simp [sinz_amo_rec] },
+  { simp [sc_amo_rec] },
   { cases ls with lit₂ ls,
-    { simp [sinz_amo_rec] },
+    { simp [sc_amo_rec] },
     { intro hamk,
       have h₁ : lit₁ ∈ lit₁ :: lit₂ :: ls, { exact mem_cons_self _ _ },
       have h₂ : lit₂ ∈ lit₁ :: lit₂ :: ls, { exact mem_cons_of_mem _ (mem_cons_self _ _) },
       cases ls with lit₃ ls,
-      { simp [sinz_amo_rec, eval_flip, literal.eval, -clause.vars_cons,
+      { simp [sc_amo_rec, eval_flip, literal.eval, -clause.vars_cons,
           aite_pos_lit (mem_vars_of_mem h₁),
           aite_pos_lit (mem_vars_of_mem h₂),
           (amz_eval_tt_iff_forall_eval_ff.mp hamk) h₁,
           (amz_eval_tt_iff_forall_eval_ff.mp hamk) h₂] },
-      { rw sinz_amo_rec,
+      { rw sc_amo_rec,
         simp [eval_flip, literal.eval, -clause.vars_cons,
           aite_pos_lit (mem_vars_of_mem h₁),
           aite_pos_lit (mem_vars_of_mem h₂),
@@ -558,38 +558,38 @@ begin
           apply cnf.eval_eq_of_agree_on,
           intros v hv,
           rcases (set.mem_union _ _ _).mp 
-            ((sinz_amo_rec_is_wb (disj_fresh_cons hdis)).2 hv) with (hv | hv),
+            ((sc_amo_rec_is_wb (disj_fresh_cons hdis)).2 hv) with (hv | hv),
           { rw [aite_pos hv, aite_pos (clause.mem_vars_cons_of_mem_vars _ hv)] },
           { rw [aite_neg (disj_right.mp (disj_fresh_cons hdis) hv.1),
                 aite_neg (disj_right.mp (disj_fresh_of_disj hdis) hv.1)] } } } } }
 end
 
-theorem sinz_amo_rec_amo {l} {g} (hdis : disj l g) : 
-  (sinz_amo_rec l g).1.eval τ = tt ∧ τ g.fresh.1 = tt → (amk 0).eval τ l.tail = tt :=
+theorem sc_amo_rec_amo {l} {g} (hdis : disj l g) : 
+  (sc_amo_rec l g).1.eval τ = tt ∧ τ g.fresh.1 = tt → (amk 0).eval τ l.tail = tt :=
 begin
   induction l with lit₁ ls ih generalizing g,
-  { simp [sinz_amo_rec], },
+  { simp [sc_amo_rec], },
   { cases ls with lit₂ ls,
-    { simp [sinz_amo_rec] },
+    { simp [sc_amo_rec] },
     { rintro ⟨heval, hfresh⟩,
       cases ls with lit₃ ls,
-      { simp [sinz_amo_rec, hfresh, eval_flip, literal.eval] at heval,
+      { simp [sc_amo_rec, hfresh, eval_flip, literal.eval] at heval,
         rw [tail, amk.eval_cons_neg heval, amk.eval_nil] },
-      { rw sinz_amo_rec at heval,
+      { rw sc_amo_rec at heval,
         simp [hfresh, eval_flip, literal.eval] at heval,
         rcases heval with ⟨h₁, h₂, h₃⟩,
         rw [tail, amk.eval_cons_neg h₂],
         exact ih (disj_fresh_of_disj (disj_of_disj_cons hdis)) ⟨h₃, h₁⟩ } } }
 end
 
-theorem sinz_amo_rec_encodes : encodes (amk 1) (sinz_amo_rec : enc_fn V) :=
+theorem sc_amo_rec_encodes : encodes (amk 1) (sc_amo_rec : enc_fn V) :=
 begin
   split,
   { intros l g hdis τ,
     induction l with lit₁ ls ih generalizing g,
-    { simp [sinz_amo_rec] },
+    { simp [sc_amo_rec] },
     { cases ls with lit₂ ls,
-      { simp [sinz_amo_rec], use τ },
+      { simp [sc_amo_rec], use τ },
       { split,
         { intro hamk,
           have h₁ : lit₁ ∈ lit₁ :: lit₂ :: ls, { exact mem_cons_self _ _ },
@@ -597,8 +597,8 @@ begin
           cases hlit₁ : lit₁.eval τ,
           { rw amk.eval_cons_neg hlit₁ at hamk,
             rcases (ih (disj_fresh_cons hdis)).mp hamk with ⟨σ, heval, hs⟩,
-            have hnmem : g.fresh.1 ∉ (sinz_amo_rec (lit₂ :: ls) g.fresh.2).1.vars,
-            { apply not_mem_form_of_is_wb sinz_amo_rec_is_wb (disj_fresh_cons hdis),
+            have hnmem : g.fresh.1 ∉ (sc_amo_rec (lit₂ :: ls) g.fresh.2).1.vars,
+            { apply not_mem_form_of_is_wb sc_amo_rec_is_wb (disj_fresh_cons hdis),
               intro hcon, rcases (set.mem_union _ _ _).mp hcon with (hv | hv),
               { exact (disj_right.mp (disj_of_disj_cons hdis) (fresh_mem_stock g)) hv },
               { exact (fresh_not_mem_fresh_stock g) hv } },
@@ -606,12 +606,12 @@ begin
             use aite (clause.vars (lit₁ :: lit₂ :: ls)) τ σ₂,
             split,
             { cases ls with lit₃ ls;
-              simp [sinz_amo_rec, eval_flip, literal.eval, -clause.vars_cons,
+              simp [sc_amo_rec, eval_flip, literal.eval, -clause.vars_cons,
                 aite_pos_lit (mem_vars_of_mem h₁), hlit₁,
                 aite_neg (disj_right.mp hdis (fresh_mem_stock g)), hfresh],
-              have : agree_on (aite (clause.vars (lit₁ :: lit₂ :: lit₃ :: ls)) τ σ₂) σ₂ (sinz_amo_rec (lit₂ :: lit₃ :: ls) g.fresh.2).1.vars,
+              have : agree_on (aite (clause.vars (lit₁ :: lit₂ :: lit₃ :: ls)) τ σ₂) σ₂ (sc_amo_rec (lit₂ :: lit₃ :: ls) g.fresh.2).1.vars,
               { intros v hv,
-                rcases mem_vars_or_stock_of_is_wb_of_mem sinz_amo_rec_is_wb (disj_fresh_cons hdis) hv with (h | h),
+                rcases mem_vars_or_stock_of_is_wb_of_mem sc_amo_rec_is_wb (disj_fresh_cons hdis) hv with (h | h),
                 { rw aite_pos (clause.mem_vars_cons_of_mem_vars _ h),
                   exact (hs _ h).symm ▸ (hs₂ _ hv) },
                 { rw aite_neg (disj_right.mp (disj_fresh_of_disj hdis) h) } },
@@ -621,7 +621,7 @@ begin
             use [aite (clause.vars (lit₁ :: lit₂ :: ls)) τ all_tt],
             split,
             { cases ls with lit₃ ls;
-              simp [sinz_amo_rec, eval_flip, literal.eval, -clause.vars_cons,
+              simp [sc_amo_rec, eval_flip, literal.eval, -clause.vars_cons,
                 aite_pos_lit (mem_vars_of_mem h₁), hlit₁,
                 aite_pos_lit (mem_vars_of_mem h₂),
                 aite_neg (disj_right.mp hdis (fresh_mem_stock g)),
@@ -629,9 +629,9 @@ begin
               { exact (amz_eval_tt_iff_forall_eval_ff.mp hamk) (mem_cons_self _ _) },
               { split,
                 { exact (amz_eval_tt_iff_forall_eval_ff.mp hamk) (mem_cons_self _ _) },
-                { rw [← sinz_amo_rec_amz (disj_fresh_of_disj (disj_of_disj_cons hdis)) hamk, cnf.eval_eq_of_agree_on],
+                { rw [← sc_amo_rec_amz (disj_fresh_of_disj (disj_of_disj_cons hdis)) hamk, cnf.eval_eq_of_agree_on],
                   intros v hv,
-                  rcases mem_vars_or_stock_of_is_wb_of_mem sinz_amo_rec_is_wb (disj_fresh_cons hdis) hv with (h | h),
+                  rcases mem_vars_or_stock_of_is_wb_of_mem sc_amo_rec_is_wb (disj_fresh_cons hdis) hv with (h | h),
                   { rw [aite_pos h, aite_pos (clause.mem_vars_cons_of_mem_vars _ h)] },
                   { rw [aite_neg (disj_right.mp (disj_fresh_of_disj hdis) h),
                         aite_neg (disj_right.mp (disj_fresh_cons hdis) h)] } } } },
@@ -642,26 +642,26 @@ begin
           { rw hlit₁ at hlit₁',
             rw amk.eval_cons_neg hlit₁',
             cases ls with lit₃ ls,
-            { simp [sinz_amo_rec, literal.eval, eval_flip, hlit₁] at heval,
+            { simp [sc_amo_rec, literal.eval, eval_flip, hlit₁] at heval,
               exact eval_singleton_pos 0 τ lit₂ },
-            { rw sinz_amo_rec at heval,
+            { rw sc_amo_rec at heval,
               simp [literal.eval, eval_flip, hlit₁] at heval,
               exact (ih (disj_fresh_cons hdis)).mpr ⟨σ, heval.2.2, (agree_on_of_agree_on_vars_cons hs)⟩ } },
           { rw hlit₁ at hlit₁',
             rw amk.eval_cons_pos hlit₁',
             cases ls with lit₃ ls,
-            { simp [sinz_amo_rec, literal.eval, eval_flip, hlit₁] at heval,
+            { simp [sc_amo_rec, literal.eval, eval_flip, hlit₁] at heval,
               rcases heval with ⟨he₁, (he₂ | he₂)⟩,
               { rw he₁ at he₂, contradiction },
               { rw ← (eval_eq_of_agree_on_of_var_mem hs 
                   (mem_vars_cons_of_mem_vars _ (mem_vars_of_mem (mem_cons_self _ _)))) at he₂,
                 rw [amk.eval_cons_neg he₂ 0 [], amk.eval_nil 0 τ] } },
             { have heval_copy := heval,
-              rw sinz_amo_rec at heval,
+              rw sc_amo_rec at heval,
               simp [literal.eval, eval_flip, hlit₁] at heval,
               rw amk.eval_eq_of_agree_on 0 (agree_on_of_agree_on_vars_cons hs),
-              exact sinz_amo_rec_amo hdis ⟨heval_copy, heval.1⟩ } } } } } },
-  { exact sinz_amo_rec_is_wb }
+              exact sc_amo_rec_amo hdis ⟨heval_copy, heval.1⟩ } } } } } },
+  { exact sc_amo_rec_is_wb }
 end
 
-end sinz_amo
+end sc_amo
